Let the function
$y(x)$
satisfy the differential equation
\begin{equation}
y''+\beta y' + \gamma y=0.
\label{60000003:vorgabe}
\end{equation}
Now set
$u(x)=e^{k x}y(x)$.
How do you have to choose $k$ and $\alpha$ so that $u$ becomes the solution
of the differential equation
\begin{equation}
u''+\alpha u=0?
\label{60000003:ziel}
\end{equation}
This problem illustrates how the first order derivatives in
\eqref{60000003:vorgabe}
can be transformed away with the help of an exponential factor
of the form $e^{kx}$.

\begin{loesung}
Let's compute the derivatives of $u$:
\begin{align*}
u'(x)&=y'(x)e^{kx}+y(x)ke^{kx}\\
u''(x)&=y''(x)e^{kx}+2y'(x)ke^{kx}+k^2y(x)e^{kx}
\end{align*}
The differential equation 
\eqref{60000003:ziel} now becomes
\[
0
=
u''(x)+\alpha u(x)
=
y''(x)e^{kx}+2y'(x)ke^{kx}+k^2y(x)e^{kx}
+ \alpha y(x)e^{kx}
=
\bigl(
y''+2k y' +(k^2+\alpha)y
\bigr)
e^{kx}
\]
This differential equation is satisfied if 
$2k=\beta$ and
$k^2+\alpha=\gamma$, thus we have to choose
\[
\begin{aligned}
k&=\frac{\beta}2
&
&\text{and}&
\alpha=\gamma-k^2=\gamma-\frac{\beta^2}4.
\end{aligned}
\]
This solution shows that the first order term of an ordinary differential
equation can be transformed away.
\end{loesung}

