Using the definition and partial integration, compute the Laplace 
transform of the function $f(t)=t$.

\begin{loesung}
The definition says
\begin{align*}
\mathscr{F}f (s)
&=
\int_0^\infty te^{-st}\,dt.
\intertext{For partial integration the factor $t$ is derived
and the factor $e^{-st}$ integrated, this leads to}
&=
\biggl[
t\frac{e^{-st}}{-s}
\biggr]_0^\infty
-
\int_0^\infty
\frac{e^{-st}}{-s}
\,dt.
\intertext{The first term vanishes as $e^{-st}\to 0$ for $t\to\infty$,
the remaining term can be integrated directly}
&=
\frac{1}{s}
\biggl[
\frac{e^{-st}}{-s}
\biggr]_0^\infty
=
\frac{1}{s}
\biggl(
-\frac{1}{-s}
\biggr)
=
\frac1{s^2}.
\qedhere
\end{align*}
\end{loesung}

