The partial differential equation
\begin{equation}
x\frac{\partial^3 u}{\partial t^3}
+\frac{\partial u}{\partial x}
=
e^{-t}
\end{equation}
on the domain
\[
\Omega
=
\{ (t,x)\in\mathbb R^2 \;|\;
t>0\text{ and } x > 0\}
\]
with boundary conditions
\[
\begin{aligned}
                                u(0,x) &= 2 &&\text{and}&
\frac{\partial   u}{\partial t  }(0,x) &= 3 &&\text{and}&
\frac{\partial^2 u}{\partial t^2}(0,x) &= 4
&&\text{for $x>0$}
\\
u(t,0)&=1
&& &&
&& &&
&&\text{for $t>0$}
\end{aligned}
\]
Use the Laplace transform with respect to the variable $t$ to convert this
problem into a family of ordinary differential equations and initial
conditions.

\begin{hinweis}
The solution of the family of ordinary differential equations is not required.
\end{hinweis}

\begin{loesung}
The Laplace transform of the right hand side of the differential equation
was computed during the lecture and is
\[
\mathcal{L}\frac{1}{\exp}(s)
=
\int_0^\infty e^{-t}e^{-st}\,dt
=
\int_0^\infty e^{-t(s+1)}\,dt
=
\biggl[-\frac1{s+1}e^{-t(s+1)}\biggr]_0^\infty
=
\frac{1}{s+1}.
\]
This means that the Laplace transform of the differential equation is
\begin{align*}
&&
\mathcal{L}\frac{\partial^3u}{\partial t^3}
+
x\mathcal{L}\frac{\partial^2u}{\partial t^2}
+
\mathcal{L}\frac{\partial u}{\partial x}
&=
\frac1{s+1}
\\
&\Rightarrow&
x\biggl(
-   \frac{\partial^2 u}{\partial t^2}(0,x)
-s  \frac{\partial   u}{\partial t  }(0,x)
-s^2                                u(0,x)
+s^3\mathcal{L}u(s,x)
\biggr)
+\frac{\partial}{\partial x}\mathcal{L}u(s,x)
&=
\frac1{s+1}
\\
&\Rightarrow&
-4x-3sx-2s^2x+xs^3\mathcal{L}u(s,x)
+\frac{\partial}{\partial x}\mathcal{L}u(s,x)
&=
\frac1{s+1}.
\end{align*}
Furthermore, we have to compute the Laplace transforms for the boundary
condition at $x=0$:
\[
\mathcal{L}1(s)
=
\int_0^\infty 1\cdot e^{-st}\,dt
=
\biggl[ -\frac1s e^{-st}\biggr]_0^\infty = \frac1s.
\]
Writing $\mathcal{L}u(s,x)=y_s(x)$, we get the family of differential
equations
\begin{align*}
y_s'(x)
+
xs^3\,y_s(x)
&=
\frac1{s+1}+4x+3sx+2s^2x
\intertext{with the initial condition}
y_s(0)
&=
\frac{1}{s}
\end{align*}
at $x=0$.
\end{loesung}



\begin{bewertung}
Laplace transform of third derivative ({\bf D}) 1 point,
usage of initial values in time ({\bf T}) 1 point,
Laplace transform of $e^{-t}$ ({\bf X}) 1 point,
Laplace transform of $1$ ({\bf 1}) 1 point,
transformed equation ({\bf E}) 1 point,
transformed initial conditions ({\bf I}) 1 point.
\end{bewertung}


