Consider the partial differential equation
\[
\frac{\partial u}{\partial x}+\frac{\partial u}{\partial t}=1
\]
on the domain $G=\{ (x,t)\,|\,t>0\}$ with boundary conditions
\[
u(x,0)=g(x).
\]
\begin{teilaufgaben}
\item
Convert this partial differential equation into a family of ordinary
differential equations using the Laplace transform on the variable $t$.
\item
Solve the partial differential equation using the method of characteristics.
\item 
Compute the Laplace transform of the solution found in b) and verify
that it is a solution of the family of ordinary differential equations
found in a).
\end{teilaufgaben}

\begin{loesung}
\begin{teilaufgaben}
\item
Applying the Laplace transform on the variable $t$ to the partial
differential equation gives the differential equation
\[
\frac{\partial}{\partial x}{\cal L}u(x,s)
+s{\cal L}u(x,s)-u(x,0)=\frac1s.
\]
The right hand side is the Laplace transform of the constant $1$, thus
\[
\int_0^\infty e^{-st}\,dt
=
\left[
-\frac1s e^{-st}
\right]_0^\infty=\frac1s.
\]
By writing $y_s(x)={\cal L}u(x,s)$ we can write the differential equation
for each $s$ as
\[
y'_s(x)+sy_s(x)-g(x)=\frac1s.
\]
\item
The characteristic curves have the differential equation
\[
\frac{d}{d\tau}\begin{pmatrix}
x\\t\\u
\end{pmatrix}
=\begin{pmatrix}
1\\1\\1
\end{pmatrix}.
\]
with the solutions
\begin{align*}
x&=\tau + x_0\\
t&=\tau + t_0\\
u&=\tau + u_0.
\end{align*}
Evaluating the boundary conditions gives
\begin{align*}
t&=\tau\\
x&=t+x_0
&\Rightarrow&x_0=x-t\\
u&=t+g(x_0)=t+g(x-t).
\end{align*}
By substituting this into the differential equation one can verify
that $u(x,t)=t+g(x-t)$ is in fact a solution:
\[
\frac{\partial u}{\partial x}+\frac{\partial u}{\partial t}
=
g'(x-t)+1-g'(x-t)=1.
\]
\item
The Laplace transform of the function $t\mapsto t+g(x-t)$ is
\[
y_s(x)=\int_0^\infty (t+g(x-t))e^{-st}\,dt.
\]
To be able to substitute this into the differential equation, we
need the derivative
\begin{align*}
y'_s(x)=\int_0^\infty g'(x-t)e^{-st}\,dt
&=\left[-g(x-t)e^{-st}\right]_0^\infty
-\int_0^\infty sg(x-t)e^{-st}\,dt
\\
&=g(x)-s\int_0^\infty g(x-t) e^{-st}\,dt.
\end{align*}
Substituting this into the differential equation we get
\begin{align*}
y'_s(x)+sy_s(x)-g(x)&=g(x)-s\int_0^\infty g(x-t)e^{-st}\,dt
\\
&\qquad
+s\int_0^\infty (t+g(x-t)) e^{-st}\,dt-g(x)
\\
&=s\int_0^\infty te^{-st}\,dt
\\
&=s\left[-\frac{t}{s}e^{-st}\right]_0^\infty
+s\int_0^\infty\frac{1}{s}e^{-st}\,dt
\\
&=\left[-\frac1s e^{-st}\right]_0^\infty
=\frac1s,
\end{align*}
so the differential equation is satisfied.
\qedhere
\end{teilaufgaben}
\end{loesung}
