Find a solution of the partial differential equation
\begin{equation}
y
\frac{\partial u}{\partial x}
+
\frac{\partial u}{\partial y}
=
3y(x^2+y)
\label{30000023:eqn}
\end{equation}
in the domain $\Omega=\{(x,y)\,|\, y>0, x\in\mathbb{R}\}$ with boundary 
condition $u(x_0,0) = x_0^3$.

\begin{loesung}
This is a quaslinear partial differential equation if first order which
can be solved using the method of characteristics.
The equations for the characteristics are:
\begin{align*}
\dot{y} &= 1
&&\Rightarrow&
y &= t+y_0 = t
\\
\dot{x} &= y
&&\Rightarrow&
x
&=
{\textstyle\frac12}t^2+x_0
&&\Rightarrow&
x_0 &= x-{\textstyle\frac12}y^2
\\
\dot{u} &= 3y(x^2+y)=3t(
({\textstyle\frac12}t^2+x_0)^2
+t)
&&\Rightarrow&
\\
&=
{\textstyle\frac34}t^5 + 3 t^3x_0 + 3tx_0^2 +3t^2
&&\Rightarrow&
u
&=
{\textstyle \frac{1}{8}} t^6
+{\textstyle\frac34}t^4x_0
+{\textstyle\frac32}t^2x_0^2 + t^3 + u_0
\\
&&&&
&=
{\textstyle \frac{1}{8}} t^6
+{\textstyle\frac34}t^4x_0
+{\textstyle\frac32}t^2x_0^2 + t^3 + x_0^3
\end{align*}
In this equation, we have to eliminate $t$ by replacing it by $y$ and
$x_0$ by replacing it by $x-\frac12y^2$.
This leads to
\begin{align}
u(x,y)
&=
\frac{1}{8}y^6
+\frac34y^4\biggl(x-\frac12y^2\biggr)
+\frac32y^2\biggl(x-\frac12y^2\biggr)^2
+y^3
+\biggl(x-\frac12y^2\biggr)^3
\notag
\\
&=
\frac1{8}y^6
+
\frac{3}{4}y^4x - \frac38y^6
+\frac32y^2x^2-\frac32y^4x +\frac{3}{8}y^6
+y^3
+x^3-\frac32x^2y^2+\frac34xy^4-\frac18y^6
\notag
\\
&=
x^3 + y^3.
\label{30000023:solution}
\end{align}
Substituting this expression in the original equation~\eqref{30000023:eqn}
and in the boundary condition shows that~\eqref{30000023:solution}
is in fact the solution.
\end{loesung}

\begin{bewertung}
Differential equations of characteristics ({\bf D}) 1 point,
solutions for $x(t)$ ({\bf X}), $y(t)$ ({\bf Y}) and $u(t)$ ({\bf U})
each 1 point,
elimination of $y_0$ using the boundary condition ({\bf E}) 1 point,
solution ({\bf S}) 1 point.
\end{bewertung}
