In problem~\ref{30000030} we have found the solution
\begin{align*}
x(t) &= e^t           \\
y(t) &= y_0Â \cosh t + f(y_0) \sinh t   \\
u(t) &= f(y_0) \cosh t + y_0 \sinh t
\end{align*}
Eliminate $t$ and $y_0$ for the boundary function $f(y_0)\equiv 0$ in order
to get a solution in the form $u = u(x,y)$.

\begin{hinweis}
$\cosh \log x = \frac12(x+1/x)$ and
$\sinh \log x = \frac12(x-1/x)$.
\end{hinweis}

\begin{loesung}
To eliminate $t$, solve the first formula for $t$ to get $t=\log x$.
Substitute into the other equations to get
\begin{align*}
y &= y_0 \frac12\biggl(x+\frac1x\biggl) = y_0\frac{x^2+1}{2x}
&&\Rightarrow &
y_0 &= \frac{2xy}{x^2+1}\\
u &= y_0 \frac12\biggl(x-\frac1x\biggl) = y_0\frac{x^2-1}{2x}
&&\Rightarrow &
u &= y\frac{x^2-1}{x^2+1}.
\qedhere
\end{align*}
\end{loesung}




