Find a solution of the partial differential equation
\begin{equation}
\frac{\partial u}{\partial x} + x\frac{\partial u}{\partial y}
=
2x(1+y)
\label{30000022:eqn}
\end{equation}
in the domain $\Omega = \{(x,y)\,|\, x >0,y\in\mathbb{R}\}$
with boundary conditions
$u(0,y_0) = y_0^2$.

\begin{loesung}
This is a quasilinear partial differential equation of first order which
can be solved using the method of characteristics.
The equations for the characteristics are:
\begin{align}
\dot{x} &= 1&&\Rightarrow&  x &= t + x_0 = t
\notag
\\
\dot{y} &= x&&\Rightarrow&  y &= {\textstyle\frac12}t^2+y_0
\notag
\\
\dot{u} &= 2x(1+y) = 2t+t^3+2ty_0
&&\Rightarrow& u &= t^2 + {\textstyle\frac14}t^4 + t^2y_0 + u_0
=
t^2+{\textstyle\frac14}t^4+t^2y_0 + y_0^2
\label{30000022:u}
\end{align}
To find the solution, $t$ and $y_0$ have to be eliminated.
This means that $t$ has to be replaced by $x$ and $y_0$ has to be
replaced by $y_0=y-\frac12x^2$.
This gives
\begin{align*}
u(x,y)
&=
x^2+{\textstyle\frac14}x^4
+x^2\bigl(y-{\textstyle\frac12}x^2\bigr)
+ \bigl(y-{\textstyle\frac12}x^2\bigr)^2
\\
&=
x^2+{\textstyle\frac14}x^4
+
x^2y
-{\textstyle\frac12}x^4
+y^2-yx^2+{\textstyle\frac14}x^4
\\
&=x^2+y^2.
\end{align*}
This completes the solution.
The characteristics of the equation~\eqref{30000022:eqn} are shown
in figure~\ref{30000022:graph}.

An alternative way to find the solution is that looking at
\eqref{30000022:u} intensly reveals that the three terms on
the right hand side of the last equation are the square of $y$,
so it follows that
\[
u(x,y) = x^2+y^2.
\]
Substituting this into the original equation \eqref{30000022:eqn}
and the boundary condition verifies that $u$ is the correct solution.
\begin{figure}
\centering
\includeagraphics[]{graph.pdf}
\caption{Characteristics of the partial differential
equation~\eqref{30000022:eqn} (red) and level curves of the solution
(blue).
\label{30000022:graph}}
\end{figure}
\end{loesung}

\begin{bewertung}
Differential equations of characteristics ({\bf D}) 1 point,
solutions for $x(t)$ ({\bf X}), $y(t)$ ({\bf Y}) and $u(t)$ ({\bf U})
each 1 point,
elimination of $y_0$ using the boundary condition ({\bf E}) 1 point,
solution ({\bf S}) 1 point.
\end{bewertung}
