Solve the partial differential equation
\[
\frac{\partial u}{\partial x}+y\frac{\partial u}{\partial y}=0
\]
on the domain
$\Omega=\{(x,y)\,|\, x> 0\}$ with boundary values
\[
u(0,y)=g(y)=y^2.
\]

\begin{loesung}
This is a quasilinear partial differential equation of first order
which can be solved using the method of characteristics.
The initial curve is given over the $y$-axis, we again denote the
$y$-values on the boundary by $y_0$.
The differential equation for the characeristics is
\[
\left.
\begin{aligned}
\dot x&=1\\
\dot y&=y\\
\dot u&=0
\end{aligned}
\right\}\quad\Rightarrow\quad
\begin{aligned}
x(y_0,t)&=t+C\\
y(y_0,t)&=De^t\\
u(y_0,t)&=u_0.
\end{aligned}
\]
The initial conditions requires that
\begin{align*}
x(y_0,0)&=0&\Rightarrow&&C&=0\\
y(y_0,0)&=y_0&\Rightarrow&&D&=y_0\\
u(y_0,0)&=y_0^2&\Rightarrow&&u_0&=y_0^2.
\end{align*}
Now we have to eliminate the variables $y_0$ and $t$ from the equations
\begin{align*}
x&=t\\
y&=y_0e^t\\
u&=y_0^2.
\end{align*}
Substituting the first and the last equation in the squared second
equation, we find
\[
y^2=ue^{2x}\qquad\Rightarrow\quad u=y^2e^{-2x}.
\]

Here is an alternative solution with a separation ansatz:
Assume the solution can be written as a product $u(x,y)=X(x)Y(y)$
and subsitute this into the partial differential equation:
\begin{align*}
X'(x)Y(y)+yX(x)Y(y)&=0\\
\Rightarrow\qquad \frac{X'(x)}{X(x)}&=-y\frac{Y'(y)}{Y(y)}.
\end{align*}
The left side depends only on $x$, the right side depends only on $y$,
so both sides must be constant, we call the constant $c$.
This leads to the two ordinary differential equations
\begin{align*}
X'(x)&=cX(x)&\Rightarrow\qquad X(x)&=K_1e^{cx}\\
Y'(y)&=\frac{c}{y}Y(y)&\Rightarrow\qquad Y(y)&=K_2y^{-c}
\end{align*}
The second equation can be solved using separation (for ordinary
differential equations).
The initial condition for $x=0$ can easily be satisfied if
$c=-2$, this gives the partial solution
\[
u(x,y)=Ke^{-2x}y^2,
\]
The initial condition for $x$ is only satisfied  if
\[
u(0,y_0)=Ky_0^2=g(y_0)\quad\Rightarrow\quad K=1,
\]
so the final solution is just as found previously
\[
u(x,y)=e^{-2x}y^2
\qedhere
\]
\end{loesung}
