Consider the partial differential equation
\begin{equation}
x \frac{\partial u}{\partial x}
+
\frac{\partial^2 u}{\partial y^2}
=
-\frac14
u
\label{40000023:eqn}
\end{equation}
on the domain 
\[
\Omega
=
\{
(x,y)\in\mathbb R^2
\;|\;
0<x<1\wedge 0<y<\pi
\}.
\]
Find a solution with boundary conditions
\[
\begin{aligned}
u(x,0) &= 0 &&\text{and}& u(x,\pi) &= 0 &&\text{for} &x&\in(0,1)
\\
u(0,y) &= 0 &&\text{and}& u(1,y) &= f(y) &&\text{for} &y&\in(0,\pi).
\end{aligned}
\]
where $f(x)$ is a triangle function with the Fourier series
\begin{align*}
f(x)
&=\begin{cases}
\displaystyle\frac{2x}{\pi}&\displaystyle\qquad 0\le x < \frac{\pi}2\\[10pt]
\displaystyle\frac{2(\pi - x)}{\pi}&\displaystyle\qquad \frac{\pi}2\le x < \pi
\end{cases}
\\
&=
\frac{8}{\pi^2}
\biggl(
\sin x - \frac1{3^2} \sin3x + \frac1{5^2}\sin5x - \frac1{7^2} \sin 7x +Â \dots
\biggr)
=
\frac{8}{\pi^2}
\sum_{k=1}^\infty \frac{(-1)^{k+1}}{(2k+1)^2} \sin (2k+1)x.
\end{align*}

\begin{hinweis}
For the dependence of the solution on $x$, try an ansatz of the form
$X(x)=x^r$ and note that only solutions with $r>0$ can be used.
\end{hinweis}

\begin{loesung}
\begin{figure}
\centering
\begin{tikzpicture}[>=latex,thick]
\node at (0,0) {\includeagraphics[width=16.8cm]{solution.jpg}};
\node at (8.3,-1.4) {$x$};
\node at (-8.3,-0.4) {$y$};
\node at (5.7,2.6) {$z$};
\end{tikzpicture}
\caption{Solution surface of the differential equation
\eqref{40000023:eqn}
\label{40000023:surface}}
\end{figure}
We use separation with the ansatz $u(x,y)=X(x)Y(y)$.
Substituting the ansatz into the equation gives
\[
x X'(x) Y(y) + X(x) Y''(y) = -\frac14 X(x)Y(y).
\]
Dividing by $X(x)Y(y)$ allows to separate the equation:
\[
x \frac{X'(x)}{X(x)} + \frac14 = - \frac{Y''(y)}{Y(y)}
\]
Since the left hand side only depends on $x$ and the right hand side only
depends on $y$, both have to be constant, we call the common constant
$\mu^2$.
We then obtain the two equations
\begin{align*}
xX'(x)&=(-{\textstyle\frac14}+\mu^2) X(x)
&&\text{and}
&
Y''(y) &= -\mu^2 Y(y)
\intertext{with homogeneous boundary conditions}
X(0)&=0
&&\text{and}
&
Y(0)&=Y(\pi)=0.
\end{align*}
The equation for $Y(y)$ has solutions $\sin(\mu y)$ and $\cos(\mu y)$.
The boundary conditions only leave $Y_k(y)=\sin ky$ where $k$ is an
integer $k>0$.
Note that $k=0$ gives the trivial solution in which we are not
interested.

For the equation for $X(x)$ we try solutions of the form $X(x)=x^r$.
Substituting this into the equation gives
\[
x rx^{r-1} = (-{\textstyle\frac14} + k^2) x^r
\]
which is only possible if $r = -\frac14 + k^2=(k+\frac12)(k-\frac12)$.
We thus obtain the functions
\[
X_k(x) = x^{-{\textstyle\frac14}+k^2}
\]
for the dependency of $x$.

Combining the factors we get solutions
\[
u_k(x,y) = X_k(x) Y_k(y) = x^{{\textstyle-\frac14}+k^2} \sin(ky)
\]
which trivially satisfies the homogeneous boundary conditions.
We have to build a linear combination that also satisfies the 
boundary condition for $x=1$, i.~e.
\begin{align*}
u(x,y)
&=
\sum_{k=1}^\infty a_k x^{-\frac14+k^2}\sin ky 
\\
\Rightarrow\qquad
u(1,y)
&=
\sum_{k=1}^\infty a_k \sin ky = f(y)
=
\frac{8}{\pi^2}
\sum_{j=1}^\infty
\frac{(-1)^{j+1}}{(2j+1)^2}
\sin (2j+1)y
\\
\Rightarrow\qquad
a_k&=\begin{cases}
\displaystyle\frac{8(-1)^{\frac{k-1}2}}{\pi^2k^2}&\qquad \text{$k$ odd}\\[10pt]
0&\qquad\text{otherwise}.
\end{cases}
\end{align*}
by comparing coefficients.
Thus the solution we are looking for is
\[
u(x,y)
=
\frac{8}{\pi^2}\sum_{j=1}^\infty (-1)^{j+1}x^{-\frac14+(2j+1)^2}\sin (2j+1) y.
\]
Figure~\ref{40000023} shows the graph of the solution $u(x,y)$.
\end{loesung}

\begin{bewertung}
Separation ansatz ({\bf S}) 1 point,
separated equations ({\bf E}) 1 point,
solution of the equation for $Y(y)$ using homogeneous boundary conditions
({\bf Y}) 1 point,
solution of the equation for $X(x)$ ({\bf X}) 1 point,
using nonhomogeneous boundary conditions to determine coefficients ({\bf C})
1 point,
solution ({\bf U}) 1 point.
\end{bewertung}





