Use a product ansatz $u(x,y) = X(x)Y(y)$ 
for the differential equation
\[
\frac{\partial^2}{\partial x \partial y} u
=
\lambda u.
\]

\begin{loesung}
Substituting into the differential equation we get
\begin{align*}
\frac{\partial}{\partial x} (X(x)Y(y))
&=
X'(x) Y(y)
\\
\frac{\partial}{\partial y} (X'(x)Y(y))
&=
X'(x)Y'(y)
\\
\Rightarrow\qquad
X'(x) Y'(y) &= \lambda X(x) Y(y).
\end{align*}
To separate, divide by $X(x)$ and by $Y'(y)$ to get
\[
\frac{X'(x)}{X(x)}
=
\lambda
\frac{Y(y)}{Y'(y)}.
\]
Both sides need to be constant so we get the two equations
\begin{align*}
\frac{X'(x)}{X(x)}&=\mu
&
\lambda\frac{Y(x)}{Y'(y)}&=\mu
\\
X'(x)&=\mu X(x)
&
Y'(x)&=\frac{\lambda}{\mu}Y(y)
\qedhere
\end{align*}
\end{loesung}
