%
% diffusion.tex -- 
%
% (c) 2019 Prof Dr Andreas Mueller, Hochschule Rapperswil
%
\section{Diffusion}
\rhead{Diffusion}
We now consider the diffusion equation in the half plane
$(t,x)\in[0,\infty)\times \mathbb R$
\[
\partial_tu-\partial_x^2u=f(t,x)
\]
with initial condition
\[
u(0,x)=g(x)\quad \forall x\in\mathbb R.
\]
We apply the transforms suited to the particular domain of definition.

\subsection{Fourier transform}
The Fourier transform or a function $g(x)$ defined on $\mathbb R$ is
defined as
\[
\hat g(k)=\frac1{\sqrt{2\pi}}\int_{\mathbb R}g(x)e^{-ikx}\,dx.
\]
The Fourier transform turns the diffusion equation and the initial
condition into
\begin{align*}
\partial_t \hat u(t,k)+k^2\hat u(t,k)&=\hat f(t,k),\\
\hat u(0,k)&=\hat g(k).
\end{align*}

\subsection{Laplace transform}
In $t$-direction, we apply the Laplace transform to get
\[
-\hat u(0,k)+(s+k^2)\mathscr{L}\hat u(s,k)=\mathscr{L}\hat f(s,k).
\]
This equation can be solved for $\mathscr{L}\hat u(s,k)$:
\[
\mathscr{L}\hat u(s,k)=\frac{\hat u(0,k)+\mathscr{L}\hat f(s,k)}{s+k^2}.
\]

\subsection{Solution of the initial value problem}
The reverse transforms can now be used to recover the solution
\begin{align*}
\hat u(t,k)&=\mathscr{L}^{-1}
\frac{\hat u(0,k)+\mathscr{L}\hat f(s,k)}{s+k^2}
\\
u(t,x)&=\mathscr{F}^{-1}\mathscr{L}^{-1}
\left(\frac{\hat u(0,k)+\mathscr{L}\hat f(s,k)}{s+k^2}\right)(t,x).
\end{align*}

