Factor the the following quadratic differential equations of first
order into two linear differential equations of first order.
\begin{teilaufgaben}
\item
$(y')^2 + 2y' - 15
=0$
\item
$(y')^2 - 4xy' + 3x^2
=0$
\item
$x(y')^2 - y' - \frac2x
=0$
\end{teilaufgaben}


\begin{loesung}
\begin{teilaufgaben}
\item 
Factoring the equation gives
\[
(y')^2 + 2y' - 15 = (y'+5)(y'-3)=0
\]
which is equivalent to the equations
\[
y'=-5
\qquad\text{and}\qquad
y'=3.
\]
\item
Factoring the equation gives
\[
(y')^2 - 4xy' + 3x^2
=
(y' - x)(y' - 3x)
=
0
\]
which is equivalent to the equations
\[
y' = x
\qquad\text{and}\qquad
y' = 3x.
\]
\item
Factoring is a little more difficult in this case, but assuming that
only integer powers the variables will appear leads to an ansatz of the
form
\[
xy'^2 - y' - \frac2x
=
(xy' + b(x))(y' + c(x)),
\]
which leads to the conditions
\[
xc(x) + b(x) = -1
\qquad\text{and}\qquad
b(x)c(x) = -\frac2x.
\]
The can be solved by choosing
\[
c(x) = \frac1x
\qquad\text{and}\qquad
b(x) = -2,
\]
giving the factorization
\[
0
=
xy'^2 - y' - \frac2x
=
(xy'-2)\biggl(y' + \frac1x\biggr)
\qquad\Rightarrow\qquad
y'=\frac2x\quad\text{and}\quad y'=-\frac1x.
\]

Alternatively, the quadratic formula can be used to solve the equation
for $y'$, giving
\[
y'(x)
=
\frac{1\pm\sqrt{1+4\cdot x\cdot \frac2x}}{2x}
=
\frac{1\pm\sqrt{1+8}}{2x}
=
\frac{1\pm3}{2x}
=
\begin{cases}
\frac2x\\
-\frac1x,
\end{cases}
\]
so the two differential equations are
\[
y'(x) = \frac2x
\qquad\text{and}\qquad
y'(x))= -\frac1x.
\]

As a third way to get the factorization, one could multiply the
equation with $x$ giving
\[
(xy')^2 -xy' - 2
=
(xy'+1)(xy'-2)
\]
which leads to the same equations.
\qedhere
\end{teilaufgaben}
\end{loesung}


